rocq-osiris/theories/program_logic/rules/stop_rules.v
@@ -787,30 +787,6 @@ Section imp_combinators.
     iApply (imp_load_block' with "Hl").
     by iIntros "!> $".
   Qed.
-  (* Ghost-based load_block: use [isBlockLocs] (persistent ghost entry) to load the block.
-     Returns the tag [t] without requiring physical block ownership. *)
-  Lemma imp_load_block_ghost' P (l : loc) ls :
-    ▷ isBlockLocs l ls -∗
-    ▷ P -∗
-    imp (load_block l) @ E <|Ψ|> ⟨⟨ ζ ⟩⟩ {{ λ '(_, ls'), ⌜ls'=ls⌝ ∗ P }}.
-  Proof.
-    iIntros "Hblock P".
-    iApply (imp_stop_load_block_ghost with "Hblock").
-    iIntros "!>" (t).
-    iApply imp_ret; first encode.
-    iFrame. done.
-  Qed.
-
-  Lemma imp_load_block_ghost (l : loc) ls :
-    ▷ isBlockLocs l ls -∗
-    imp (load_block l) @ E <|Ψ|> ⟨⟨ ζ ⟩⟩ {{ λ '(t', ls'), ⌜ls' = ls⌝ }}.
-  Proof.
-    iIntros "#Harr".
-    iApply (imp_stop_load_block_ghost with "Harr").
-    iIntros "!>" (t).
-    iApply imp_ret; first encode.
-    done.
-  Qed.
 
   (* ------------------------------------------------------------------------ *)
   (* [CExchange]. *)
@@ -988,6 +964,39 @@ Section imp_combinators.
   Qed.
 
 End imp_combinators.
+
+Section polymorphic_combinators.
+
+  Context `{!osirisGS Σ}.
+  Context {E : coPset} {Ψ : iEff Σ}.
+  Context {X : Type} {ζ : X → iProp Σ}.
+
+  (* Ghost-based load_block: use [isBlockLocs] (persistent ghost entry) to load the block.
+     Returns the tag [t] without requiring physical block ownership. *)
+  Lemma imp_load_block_ghost' P (l : loc) ls :
+    ▷ isBlockLocs l ls -∗
+    ▷ P -∗
+    imp (load_block l) @ E <|Ψ|> ⟨⟨ ζ ⟩⟩ {{ λ '(_, ls'), ⌜ls'=ls⌝ ∗ P }}.
+  Proof.
+    iIntros "Hblock P".
+    iApply (imp_stop_load_block_ghost with "Hblock").
+    iIntros "!>" (t).
+    iApply imp_ret; first encode.
+    iFrame. done.
+  Qed.
+
+  Lemma imp_load_block_ghost (l : loc) ls :
+    ▷ isBlockLocs l ls -∗
+    imp (load_block l) @ E <|Ψ|> ⟨⟨ ζ ⟩⟩ {{ λ '(t', ls'), ⌜ls' = ls⌝ }}.
+  Proof.
+    iIntros "#Harr".
+    iApply (imp_stop_load_block_ghost with "Harr").
+    iIntros "!>" (t).
+    iApply imp_ret; first encode.
+    done.
+  Qed.
+
+End polymorphic_combinators.
 
 Section imp_concurrent_combinators.
 
